Started proving invariants about covers

src/RqRsInvAtomic.v
@@ -1,8 +1,9 @@
 Require Import Peano_dec Omega List ListSupport.
 Require Import Common FMap.
-Require Import Syntax Semantics SemFacts StepM Invariant Serial.
+Require Import Syntax Semantics SemFacts StepM Invariant Serial SerialFacts.
 Require Import Reduction Commutativity QuasiSeq Topology.
-Require Import RqRsTopo RqRsFacts RqRsInvMsg.
+Require Import RqRsTopo RqRsFacts RqRsInvMsg RqRsInvLock.
+Require Import RqUpRed.
 
 Set Implicit Arguments.
 
@@ -36,66 +37,321 @@ Proof.
   induction 1; simpl; intros; eauto.
 Qed.
 
-Section Covers.
+Section RqUpStart.
   Context {oifc: OStateIfc}.
   Variables (dtr: DTree)
             (sys: System oifc).
 
   Hypothesis (Hrrs: RqRsSys dtr sys).
+  
+  Definition NonRqUpL (lbl: MLabel) :=
+    match lbl with
+    | RlblEmpty _ => True
+    | RlblIns _ => True
+    | RlblOuts _ => True
+    | RlblInt oidx _ _ routs => ~ RqUpMsgs dtr oidx routs
+    end.
 
-  Definition RqUpCoverInv (oinds: list IdxT) (rqUp: Id Msg) :=
-    forall ruFrom ruTo,
+  Ltac disc_NonRqUpL :=
+    repeat
+      match goal with
+      | [ |- NonRqUpL _] => red
+      | [ |- ~ RqUpMsgs _ _ _] => let Hx := fresh "H" in intro Hx
+      | [H: RqUpMsgs _ _ _ |- _] =>
+        let cidx := fresh "cidx" in
+        let rqUp := fresh "rqUp" in
+        destruct H as [cidx [rqUp ?]]; dest
+      | [H: _ :: _ = _ :: _ |- _] => inv H; simpl in *
+      end.
+
+  Ltac disc_rule_custom ::=
+    try disc_footprints_ok.
+
+  Lemma rqUp_start_ok_base:
+    forall st1 st2 oidx ridx rins routs,
+      Reachable (steps step_m) sys st1 ->
+      step_m sys st1 (RlblInt oidx ridx rins routs) st2 ->
+      (exists roidx, RqUpMsgs dtr roidx routs) \/
+      NonRqUpL (RlblInt oidx ridx rins routs).
+  Proof.
+    destruct Hrrs as [? [? ?]]; intros.
+    pose proof (footprints_ok H0 H2).
+    inv_step.
+    good_rqrs_rule_get rule.
+    good_rqrs_rule_cases rule.
+
+    - disc_rule_conds.
+      right; disc_NonRqUpL.
+      solve_midx_false.
+    - disc_rule_conds.
+      right; disc_NonRqUpL.
+      solve_midx_false.
+
+    - disc_rule_conds.
+      + left.
+        pose proof (rqEdgeUpFrom_Some H _ H6).
+        destruct H14 as [rsUp [down [pidx ?]]]; dest.
+        eexists; red.
+        do 2 eexists; eauto.
+      + right; disc_NonRqUpL; subst.
+        eapply RqRsDownMatch_rq_rs in H20; [|left; reflexivity].
+        destruct H20 as [rcidx [rsUp ?]]; dest.
+        solve_midx_false.
+      + right; disc_NonRqUpL; subst.
+        eapply RqRsDownMatch_rq_rs in H6; [|left; reflexivity].
+        destruct H6 as [rcidx [rsUp ?]]; dest.
+        solve_midx_false.
+
+    - good_footprint_get (obj_idx obj).
+      disc_rule_conds.
+      + right; disc_NonRqUpL.
+        rewrite H11 in H25; discriminate.
+      + right; disc_NonRqUpL.
+        rewrite H8 in H23; discriminate.
+      + right; disc_NonRqUpL.
+        rewrite H8 in H20; discriminate.
+
+    - disc_rule_conds.
+      right; disc_NonRqUpL; subst.
+      eapply RqRsDownMatch_rq_rs in H20; [|left; reflexivity].
+      destruct H20 as [rcidx [rsUp ?]]; dest.
+      solve_midx_false.
+  Qed.
+
+  Lemma rqUp_start_ok_end:
+    forall rqUp cidx roidx inits ruins pruhst ruouts,
       msg_type (valOf rqUp) = MRq ->
-      parentIdxOf dtr ruFrom = Some ruTo ->
-      rqEdgeUpFrom dtr ruFrom = Some (idOf rqUp) ->
-      SubList oinds (subtreeIndsOf dtr ruFrom).
+      parentIdxOf dtr cidx = Some roidx ->
+      rqEdgeUpFrom dtr cidx = Some (idOf rqUp) ->
+      Atomic msg_dec inits ruins pruhst ruouts [rqUp] ->
+      forall oidx ridx routs st1 st2,
+        Reachable (steps step_m) sys st1 ->
+        step_m sys st1 (RlblInt oidx ridx [rqUp] routs) st2 ->
+        exists ruhst nhst,
+          RlblInt oidx ridx [rqUp] routs :: pruhst = nhst ++ ruhst /\
+          (ruhst = nil \/
+           (exists roidx0 rqUps ruins0 ruouts0,
+               RqUpMsgs dtr roidx0 rqUps /\
+               Atomic msg_dec inits ruins0 ruhst ruouts0 rqUps /\
+               (nhst = nil \/
+                (exists nins nouts, Atomic msg_dec rqUps nins nhst nouts routs)))) /\
+          Forall NonRqUpL nhst.
+  Proof.
+    destruct Hrrs as [? [? ?]]; intros.
+    pose proof (footprints_ok H0 H6).
+    inv_step.
+    good_rqrs_rule_get rule.
+    good_rqrs_rule_cases rule.
 
-  Definition RqDownCoverInv (oinds: list IdxT) (rqDown: Id Msg) :=
-    forall rdFrom rdTo,
-      msg_type (valOf rqDown) = MRq ->
-      parentIdxOf dtr rdTo = Some rdFrom ->
-      edgeDownTo dtr rdTo = Some (idOf rqDown) ->
-      DisjList oinds (subtreeIndsOf dtr rdTo).
+    - disc_rule_conds.
+      eexists pruhst, [_].
+      repeat ssplit.
+      + reflexivity.
+      + right; do 4 eexists.
+        repeat ssplit; try eassumption.
+        * red; do 2 eexists.
+          repeat ssplit; eauto.
+        * right; do 2 eexists.
+          econstructor.
+      + constructor; [|constructor].
+        disc_NonRqUpL; subst.
+        rewrite H9 in H12; discriminate.
 
-  Definition RsUpCoverInv (oinds: list IdxT) (rsUp: Id Msg) :=
+    - exfalso; disc_rule_conds.
+      solve_midx_false.
+
+    - disc_rule_conds.
+      + eexists (_ :: pruhst), nil.
+        repeat ssplit.
+        * reflexivity.
+        * right.
+          pose proof (rqEdgeUpFrom_Some H _ H11).
+          destruct H7 as [rsUp [down [pidx ?]]]; dest.
+          exists pidx, [(rqTo, rqtm)]; do 2 eexists.
+          repeat ssplit.
+          { red; do 2 eexists.
+            repeat ssplit; eauto.
+          }
+          { econstructor; try reflexivity; try eassumption.
+            { discriminate. }
+            { apply SubList_refl. }
+            { rewrite removeL_nil; reflexivity. }
+          }
+          { left; reflexivity. }
+        * constructor.
+      + eexists pruhst, [_].
+        repeat ssplit.
+        * reflexivity.
+        * right; do 4 eexists.
+          repeat ssplit; try eassumption.
+          { red; do 2 eexists.
+            repeat ssplit; eauto.
+          }
+          { right; do 2 eexists.
+            econstructor.
+          }
+        * constructor; [|constructor].
+          disc_NonRqUpL; subst.
+          eapply RqRsDownMatch_rq_rs in H27; [|left; reflexivity].
+          destruct H27 as [rcidx [rsUp ?]]; dest.
+          solve_midx_false.
+      + exfalso; solve_midx_false.
+
+    - exfalso; disc_rule_conds.
+    - exfalso; disc_rule_conds.
+  Qed.
+
+  Lemma rqUp_start_ok:
+    forall inits ins hst outs eouts,
+      Atomic msg_dec inits ins hst outs eouts ->
+      forall st1 st2,
+        Reachable (steps step_m) sys st1 ->
+        steps step_m sys st1 hst st2 ->
+        exists ruhst nhst,
+          hst = nhst ++ ruhst /\
+          (ruhst = nil \/
+           exists roidx rqUps ruins ruouts,
+             RqUpMsgs dtr roidx rqUps /\
+             Atomic msg_dec inits ruins ruhst ruouts rqUps /\
+             (nhst = nil \/
+              exists nins nouts, Atomic msg_dec rqUps nins nhst nouts eouts)) /\
+          Forall NonRqUpL nhst.
+  Proof.
+    destruct Hrrs as [? [? ?]].
+    induction 1; simpl; intros; subst.
+
+    - inv_steps.
+      eapply rqUp_start_ok_base in H9; [|eassumption].
+      destruct H9.
+      + destruct H3 as [roidx ?].
+        eexists; exists nil.
+        repeat ssplit.
+        * reflexivity.
+        * right; do 4 eexists.
+          repeat ssplit; eauto.
+          econstructor.
+        * constructor.
+      + exists nil; eexists.
+        repeat ssplit.
+        * rewrite app_nil_r; reflexivity.
+        * left; reflexivity.
+        * constructor; auto.
+
+    - inv_steps.
+      specialize (IHAtomic _ _ H8 H10).
+      destruct IHAtomic as [pruhst [pnhst ?]]; dest; subst.
+      destruct H6; subst.
+
+      + exists nil.
+        exists (RlblInt oidx ridx rins routs :: pnhst).
+        repeat rewrite app_nil_r in *.
+        repeat ssplit.
+        * reflexivity.
+        * left; reflexivity.
+        * constructor; [|assumption].
+          (*
+           * 1) [Atomic msg_dec inits ins pnhst outs eouts] ->
+           *    [Forall NonRqUpL pnhst] ->
+           *    [eouts] does not have any RqUps.
+           * 2) [SubList rins eouts] -> [rins] does not have any RqUps.
+           * 3) NonRqUpL (RlblInt oidx ridx rins routs)
+           *)
+          admit.
+
+      + destruct H5 as [roidx [rqUps [ruins [ruouts ?]]]]; dest.
+        destruct H9; subst.
+
+        * simpl in *.
+          pose proof (atomic_unique H2 H6); dest; subst; clear H2.
+          red in H5; destruct H5 as [cidx [rqUp ?]]; dest; subst.
+          assert (rins = [rqUp]); subst.
+          { inv_step; inv H23.
+            destruct rins; [elim H3; reflexivity|].
+            pose proof (H4 i (or_introl eq_refl)); Common.dest_in.
+            destruct rins; [reflexivity|].
+            specialize (H4 i0 (or_intror (or_introl eq_refl))); Common.dest_in.
+            red in H12; simpl in H12.
+            inv H12; elim H15; left; reflexivity.
+          }
+          pose proof (reachable_steps H8 H10).
+          rewrite removeL_nil; simpl.
+          eapply rqUp_start_ok_end; eauto.
+
+        * destruct H9 as [pnins [pnouts ?]].
+          exists pruhst, (RlblInt oidx ridx rins routs :: pnhst).
+          repeat ssplit.
+          { reflexivity. }
+          { right; exists roidx, rqUps, ruins, ruouts.
+            repeat ssplit; try assumption.
+            right; do 2 eexists.
+            econstructor; eauto.
+          }
+          { constructor; [|assumption].
+            (*
+             * 1) [Atomic msg_dec inits ins pnhst outs eouts] ->
+             *    [Forall NonRqUpL pnhst] ->
+             *    [eouts] does not have any RqUps.
+             * 2) [SubList rins eouts] -> [rins] does not have any RqUps.
+             * 3) NonRqUpL (RlblInt oidx ridx rins routs)
+             *)
+            admit.
+          }
+  Admitted.
+
+End RqUpStart.
+
+Section Covers.
+  Context {oifc: OStateIfc}.
+  Variables (dtr: DTree)
+            (sys: System oifc).
+  Hypothesis (Hrrs: RqRsSys dtr sys).
+
+  Definition WellUpLocked (rqUps: MHistory) (orqs: ORqs Msg) :=
     True.
 
-  Definition RsDownCoverInv (oinds: list IdxT) (rsDown: Id Msg) :=
-    forall rdFrom rdTo,
-      msg_type (valOf rsDown) = MRs ->
-      parentIdxOf dtr rdTo = Some rdFrom ->
-      edgeDownTo dtr rdTo = Some (idOf rsDown) ->
-      DisjList oinds (subtreeIndsOf dtr rdTo).
+  Section OnWellUpLocked.
+    Variables (rqUps: MHistory) (orqs: ORqs Msg).
+    Hypothesis (Hwul: WellUpLocked rqUps orqs).
+  
+    Definition RqDownCoverInv (rqDown: Id Msg) (hst: MHistory) :=
+      forall rdFrom rdTo,
+        msg_type (valOf rqDown) = MRq ->
+        parentIdxOf dtr rdTo = Some rdFrom ->
+        edgeDownTo dtr rdTo = Some (idOf rqDown) ->
+        DisjList (oindsOf hst) (subtreeIndsOf dtr rdTo).
 
-  Definition CoverInvMsg (oinds: list IdxT) (eout: Id Msg) :=
-    RqUpCoverInv oinds eout /\
-    RqDownCoverInv oinds eout /\
-    RsUpCoverInv oinds eout.
+    (* Definition RsUpCoverInv (hoinds: list IdxT) (rsUp: Id Msg) := *)
 
-  Definition CoverInv (oinds: list IdxT) (eouts: list (Id Msg)) :=
-    Forall (CoverInvMsg oinds) eouts.
+    Definition RsDownCoverInv (rsDown: Id Msg) (hst: MHistory) :=
+      forall rdFrom rdTo,
+        msg_type (valOf rsDown) = MRs ->
+        parentIdxOf dtr rdTo = Some rdFrom ->
+        edgeDownTo dtr rdTo = Some (idOf rsDown) ->
+        DisjList (oindsOf hst)
+                 (removeL eq_nat_dec (subtreeIndsOf dtr rdTo) (oindsOf rqUps)).
+
+    Definition MsgOutCoverInv (eout: Id Msg) (hst: MHistory) :=
+      RqDownCoverInv eout hst /\
+      RsDownCoverInv eout hst.
+
+    Definition MsgOutsCoverInv (eouts: list (Id Msg)) (hst: MHistory) :=
+      Forall (fun eout => MsgOutCoverInv eout hst) eouts.
+
+  End OnWellUpLocked.
 
   Ltac disc_rule_custom ::=
     try disc_footprints_ok.
   
-  (* Lemma cover_inv: *)
+  (* Lemma covers_ok: *)
   (*   forall inits ins hst outs eouts, *)
   (*     Atomic msg_dec inits ins hst outs eouts -> *)
   (*     forall s1 s2, *)
   (*       Reachable (steps step_m) sys s1 -> *)
   (*       steps step_m sys s1 hst s2 -> *)
-  (*       CoverInv (oindsOf hst) eouts. *)
+  (*       LockCoverInv (oindsOf hst) s2.(bst_orqs) /\ *)
+  (*       MsgOutsCoverInv (oindsOf hst) eouts. *)
   (* Proof. *)
-  (*   destruct Hrrs as [? [? ?]]. *)
-  (*   induction 1; simpl; intros. *)
-
-  (*   - inv_steps; inv_step. *)
-  (*     admit. *)
-  (*     (* good_rqrs_rule_get rule. *) *)
-  (*     (* good_rqrs_rule_cases rule. *) *)
-
-
-  (*   - inv_steps; inv_step. *)
+  (* Qed. *)
 
 End Covers.
 
